<?xml version="1.0" encoding="UTF-8"?>

<section xml:id="sec-polys" xmlns:xi="http://www.w3.org/2001/XInclude">
  <title>The minimal polynomial</title>

  <introduction>
    <p> This section will describe some important properties about
    polynomials and demonstrate how they might help us understand linear
    transformations.  
    </p>
    
    <p> We will begin by studying familiar polynomials, such as you
    saw in high school algebra.  For example, <m>p(x)=2x^2 - 3x + 7</m>
    is a quadratic polynomial.  Eventually, we will consider polynomials
    evaluated on an operator <m>T</m>.  For instance,
    evaluating <m>p(x)</m> on the operator <m>T</m> produces a new
    operator
    <m>p(T) = 2T^2 - 3T + 7I</m>.  As a preview for how this may be
    useful, the polynomial <m>p(x)=x-2</m> leads to the operator
    <m>p(T) = T-2I</m> whose null space is the set of eigenvectors
    associated to the eigenvalue <m>\lambda = 2</m>.
    </p>
  </introduction>
  
  <subsection>
    <title>Properties of Polynomials</title>

    <p>We will be interested in polynomials that depend on a single
    variable, which will often be <m>x</m>.  
    A general polynomial has
    the form
    <me>
      p(x)=a_nx^n + a_{n-1}x^{n-1}+\ldots + a_1x+a_0
    </me>
    where <m>a_j</m> are the <em>coefficients</em> of <m>p(x)</m> and
    are elements in either <m>\field=\C</m> or
    <m>\real</m>.
    </p>

    <p>The <em>degree</em> of a polynomial is the highest power of
    <m>x</m> whose coefficient is nonzero.  For example, the degree of
    <me>
      p(x)=-2x^7 + 4x^6 -x^5 + 4x^3-3x + 1
    </me>
    is <m>\deg(p) = 7</m>.
    </p>

    <p> We have already seen that the set of polynomials form a vector
    space, which means we can multiply polynomials by scalars
    and we can add them.  An additional operation allows us to
    multiply two polynomials 
    together.
    </p>

    <example xml:id="example-poly-product">
      <statement>
        <p>Suppose that <m>p(x)=3x^2-4x+2</m> and <m>q(x)=8x-5</m>.
        We multiply polynomials term by term so that
        <me>
	  (pq)(x) = 24x^3-27x^2+36x-10
        </me>
        More generally, denoting the coefficients of <m>p</m> by
        <m>a_j</m> and the coefficients of <m>q</m> by <m>b_j</m>, the
        coefficients of <m>pq</m> are
        <me xml:id="me-poly-mult">
	  c_k=\sum_{j=0}^k a_jb_{k-j}=\sum_{j=0}^k b_ja_{k-j}
          </me>.
        </p>
      </statement>
    </example>

    <assemblage>
      <title>Properties of polynomial multiplication</title>
      <p>Two important properties follow from the general expression
      for the coefficients of the product given in
      <xref ref="example-poly-product"/>.
      First, the order in which we multiply
      polynomials is irrelevant;  that is,
      <me>pq = qp</me>.
      </p>
      
      <p>Second, the degree of the product is the sum of the degrees;
      that is,
      <me>
        \deg(pq)=\deg(p)+\deg(q)
        </me>.
      </p>
    </assemblage>
      
    <p>Integers satisfy a property often called the <em>Division
    Algorithm</em>.  Suppose that <m>a</m> and <m>b</m> are positive
    integers.  Then there are integers <m>q</m> and <m>r</m> such that
    <me>
      a = bq + r
    </me>
    where <m>0\leq r \leq b-1</m>.  We say that <m>q</m> is the
    <em>quotient</em> and <m>r</m> is the <em>remainder</em>.  For
    example, if 
    <m>a=17</m> and <m>b=5</m>, then
    <me>
      17 = 3\cdot5 + 2
    </me>.
    </p>

    <p>Polynomials satisfy a similar property also called the Division
    Algorithm as given in the following proposition.
    </p>

    <proposition xml:id="prop-poly-division">
      <title>The Division Algorithm</title>
      <statement>
	<p>If <m>p(x)</m> and <m>s(x)</m> are polynomials, then there
	are unique polynomials <m>q(x)</m> and <m>r(x)</m> such that
	<me>
	  p(x) = (qs)(x) + r(x)
	</me>
	where <m>\deg(r) \lt \deg(s)</m>.
	</p>
      </statement>
    </proposition>
    
    <example>
      <statement>
	<p>Rather than proving the Division Algorithm for polynomials,
	we will illustrate with an example.  Suppose that
	<m>p(x)=6x^3 + x^2 - 17x + 8</m> and <m>s(x)=2x^2 + 2x -
	1</m>.
	</p>

	<p>To get started, let's consider the highest degree terms in
	both polynomials.  For <m>p(x)</m>, it is <m>6x^3</m> while
	for <m>s(x)</m>, it is <m>2x^2</m>.  We'd like to multiply
	<m>s(x)</m> by something to get close to <m>p(x)</m>. Since
	the ratio of the highest degree terms is <m>3x</m>, we
	multiply <m>s(x)</m> by <m>3x</m>, which gives
	<me>
	  p(x) - (3x)s(x) = -8x^2 - 14x + 8
	</me>.
	</p>

	<p>Now we ask what we should multiply by <m>s(x)</m> to
	realize the <m>-8x^2</m> term.  Since the highest degree term of
	<m>s(x)</m> is <m>2x^2</m>, we multiply by <m>-4</m>.  This
	means that
	<me>
	  p(x) - (3x-4)s(x) = -2x+4
	</me>.
	Since the highest degree term of <m>s(x)</m> is <m>2x^2</m>,
	there is nothing we can multiply by <m>s(x)</m> to realize the
	highest degree term of the right hand side.
	This means that we have
	<me>
	  p(x) = (3x-4)s(x) + (-2x+4)
	</me>
	so the quotient is <m>q(x)=3x-4</m> and the remainder is
	<m>r(x)=-2x+4</m>. 
	</p>

	<p>This algorithm is sometimes called <em>synthetic
	division</em> and is sometimes taught in high school.  We
	won't be actually be implementing this algorithm, but this
	example is meant to illustrate why <xref
	ref="prop-poly-division"/> is true.  Implementing this
	algorithm for general polynomials will give a proof of the
	Division Algorithm.
	</p>
      </statement>
    </example>

    <p>One important implication of the Division Algorithm is the
    following fact that we will use quite a bit.  Remember that a root
    <m>\lambda</m> of a polynomial is a value for which
    <m>p(\lambda)=0</m>. 
    </p>

    <proposition xml:id="prop-root-factor">
      <statement> If <m>\lambda</m> is a root of the polynomial <m>p(x)</m>,
      then
      <me>
	p(x)=(x-r)q(x)
      </me>
      for some polynomial <m>q</m>.
      </statement>

      <proof>
	<p>The Division Algorithm tells us that
	<me>p(x)=(x-\lambda)q(x) + r(x)
	</me>.
	In the notation of the Division Algorithm,
	<m>s(x)=x-\lambda</m> and <m>\deg(r) \lt \deg(s) = 1</m>.
	Therefore <m>\deg(r)=0</m>, which means that <m>r(x)</m> is a
	constant <m>r</m>.
	</p>

	<p>Now we know that <m>0=p(\lambda)=(\lambda-\lambda)q(\lambda)+r =
	r</m>, which says that <m>r=0</m>.  Therefore, we have
	<me>
	  p(x)=(x-\lambda)q(x)
	</me>.
	</p>
      </proof>
    </proposition>

    <p>This proposition shows that there is a relationship between the
    factors of a polynomial <m>p(x)</m> and its roots.  Polynomials
    with complex coefficients are special because the Fundamental
    Theorem of Algebra tells us that every such polynomial has a
    root.  The proof of this theorem is outside the scope of our
    course, but students often see it in a course in complex analysis.
    </p>

    <theorem xml:id="thm-fta">
      <title>Fundamental Theorem of Algebra</title>

      <statement>
	<p>If <m>p(x)</m> is a degree <m>n</m> polynomial having
	complex coefficients, then there are <m>n</m> roots,
	<m>\lambda_1, \lambda_2, \ldots, \lambda_n</m>, possibly with
	repitition.  This means that
	<me>p(x)=a_n(x-\lambda_1)(x-\lambda_2)\ldots(x-\lambda_n)
	</me>.
	</p>
      </statement>
    </theorem>

    <p>While this important theorem only holds for polynomials with
    complex coefficients, we can deduce something about polynomials
    with real coefficients.  For instance, if <m>p(x)</m> is a
    polynomial with real coefficients and <m>\lambda</m> is a complex,
    non-real 
    root, then so is its complex conjugate <m>\overline{\lambda}</m>.
    This follows because
    <me>
      0=\overline{p(\lambda)} = p(\overline{\lambda})
    </me>.
    We have <m>(x-\lambda)(x-\overline{\lambda}) = x^2+bx + c</m> where
    <m>b = -(\lambda+\overline{\lambda})</m> and
    <m>c=\lambda\overline{\lambda}</m>.  Since this quadratic
    polynomial does not have real roots, we know from the quadratic
    formula that <m>b^2\lt 4ac</m>.  Therefore,
    </p>

    <proposition>
      <statement>
	<p>If <m>p(x)</m> is a polynomial with real coefficients,
	there are real roots <m>\lambda_1,\ldots,\lambda_m</m> such
	that 
	<me>
	  p(x)=a_n(x-\lambda_1)\ldots(x-\lambda_r)(x^2+b_1x+c_1^2)\ldots(x^2+b_sx+c_s)
	  </me>.
	</p>
      </statement>
    </proposition>
  </subsection>

  <subsection>
    <title>The minimal polynomial of an operator</title>

    <p>As mentioned in the introduction to this section, our interest
    in polynomials stems from the insights we gain when we evaluate a
    polynomial on an operator <m>T</m>.  For instance, if
    <m>p(x)=x^2+4x-5</m>, then <m>p(T) = T^2 + 4T - 5I</m> a new
    operator.  Notice 
    that we consider the constant term to be multiplied by the
    identify transformation <m>I</m>.
    </p>

    <definition>
      <statement>
        <p>If <m>W</m> is a vector subspace of <m>V</m> and <m>T:V\to
        V</m> an operator, we say that <m>W</m> is <em>invariant</em>
        under <m>T</m> if <m>T(\wvec)\in W</m> for all <m>\wvec\in
        W</m>.
        </p>
      </statement>
    </definition>

    <p>Remember that the order in which we multiply polynomials is not
    important.  In particular, <m>p(T)q(T)=q(T)p(T)</m>.  This leads
    to the following important proposition.
    </p>

    <proposition>
      <statement>
	<p>If <m>p(x)</m> is a polynomial and <m>T</m> an operator,
	then both <m>\nul(p(T))</m> and <m>\range(p(T))</m> are
	invariant subspaces under <m>T</m>.
	</p>
      </statement>

      <proof>
	<p> Suppose that <m>\vvec</m> is in <m>\nul(p(T))</m>, which
	means that <m>p(T)\vvec = \zerovec</m>.  We need to explain
	why <m>T\vvec</m> is also in <m>\nul(p(T))</m>, which leads us
        to 
	<me>
	  p(T)T\vvec = Tp(T)\vvec = T\zerovec = \zerovec
	</me>.
	</p>

	<p>Similarly, if <m>\vvec</m> is in <m>\range(p(T))</m>, then
	there is a vector <m>\uvec</m> so that
	<m>\vvec=p(T)\uvec</m>.  Then
	<me>
	  T\vvec = Tp(T)\uvec = p(T)(T\uvec)
	</me>,
	which shows that <m>T\vvec</m> is also in
	<m>\range(p(T))</m>.  Therefore, <m>\range(p(T))</m> is an
	invariant subspace of <m>T</m>.
	</p>
      </proof>
    </proposition>

    <p>We now come to a crucial result for our upcoming explorations.
    First, we need to make the following definition clear.
    </p>

    <definition>
      <statement>A <em>monic</em> polynomial is a polynomial where the
      coefficient of the highest degree term is <m>1</m>.
      </statement>
    </definition>

    <p>For instance, <m>x^5 - x^4 + 3x - 2</m> is a monic polynomial,
    but <m>3x^3+2x-1</m> is not.
    </p>

    <theorem xml:id="thm-minimal-polynomial">
      <title>The minimal polynomial of an operator</title>

      <statement>
	<p>Suppose that <m>V</m> is a finite-dimensional vector space over
	either <m>\C</m> or <m>\R</m> and that <m>T</m> is an operator
	on <m>V</m>.  There is a unique monic polynomial <m>p</m> of
	smallest degree such that <m>p(T)=0</m>.  Moreover,
	<m>\deg(p)\leq \dim(V)</m>.  We call this polynomial the
	<em>minimal polynomial</em> of <m>T</m>.
	</p>
      </statement>

      <proof>
	<p>Our proof proceeds by induction on the dimension of
	<m>V</m>.  To begin, suppose that <m>\dim(V) = 1</m>, which
	means that <m>V=\laspan{\vvec}</m> for some vector
	<m>\vvec</m>.  Then <m>T\vvec = \lambda\vvec</m> for some
	<m>\lambda</m>, which is possibly <m>0</m>.  Then
	<m>(T-\lambda I)\vvec = \zerovec</m>, which means that
	<m>T-\lambda I = 0</m> since <m>\vvec</m> spans <m>V</m>.
	Therefore, if <m>p(x) = x-\lambda</m>, we have <m>p(T)=0</m>.
	</p>

	<p>We now imagine that <m>\dim(V)=n</m> and that the theorem
	has been verified for all operators on vector spaces of
	dimension less than <m>n</m>.  We choose a vector <m>\vvec</m>
	and consider the powers <m>T^k\vvec</m>;  that is, consider
	the vectors
	<me>
	  \vvec,T\vvec,T^2\vvec,\ldots,T^n\vvec
	</me>.
	Since there are <m>n+1</m> vector in this set and
	<m>\dim(V)=n</m>, we know this is a linearly independent set.
	</p>

	<p>Choose <m>m</m> to be the smallest integer such that
	<m>T^m\vvec</m> is a linear combination of
	<m>\vvec,T\vvec,\ldots,T^{m-1}\vvec</m>.  This means two
	things.  First, the vectors
	<m>\vvec,T\vvec,\ldots,T^{m-1}\vvec</m> are linearly
	independent.  Second, there are constants
	<me>
	  a_0\vvec + a_1T\vvec + \ldots + a_{m-1}T^{m-1}\vvec +
	  T^m\vvec = \zerovec
	</me>.
	If we define the degree <m>m</m> monic polynomial
	<me>
	  p(x)=a_0 + a_1x + \ldots + a_{m-1}x^{m-1}+x^m
	</me>,
	then <m>p(T)\vvec = \zerovec</m>.  That is, <m>\vvec</m> is in
	<m>\nul(p(T))</m>.
	</p>

	<p>Since <m>\nul(p(T))</m> is invariant under <m>T</m> and
	<m>\vvec</m> is in <m>\nul(p(T))</m>, we know that
	<me>
	  \vvec,T\vvec,\ldots,T^{m-1}\vvec
	</me> 
	are all in <m>\nul(p(T))</m>.  These vectors are linearly
	independent so we know that <m>\dim(\nul(p(T)))\geq m</m>.
	Therefore,
	<me>
	  \dim(\range(p(T))) = \dim(V) - \dim(\nul(p(T))) \leq n - m
	</me>.
	</p>

	<p>For convenience, we will denote the vector space
	<m>W=\range(p(T))</m>.  Since <m>W</m> is invariant under
	<m>T</m>, <m>T</m> is an operator on <m>W</m>, whose dimension
	is less than <m>\dim(V)</m>.  By the induction hypothesis, we
	know that there is a unique monic polynomial <m>q(x)</m> such
	that <m>q(T|_W)=0</m>.  Again by the induction hypothesis, it
	also follows that <m>\deg(q) \leq \dim(W) \leq n - m</m>.
	</p>

	<p>Now consider the polynomial <m>pq</m> whose degree is
	<me>
	  \deg(qp) = \deg(q)+\deg(p) \leq n - m + m \leq n = \dim(V)
	</me>.
	Moreover, both <m>p</m> and <m>q</m> are monic so <m>pq</m> is
	also monic.  Finally, for any vector <m>\vvec</m> in <m>V</m>,
	we have 
	<me>
	  (qp)(T)\vvec = q(T)p(T)\vvec = q(T)(p(T)\vvec) = \zerovec
	</me>
	where the last equality holds because <m>p(T)\vvec</m> is in
	<m>W=\range(p(T))</m> and <m>q(T)\uvec=\zerovec</m> for any
	vector <m>\uvec</m> in <m>W</m>.  Since
	<m>(qp)(T)\vvec=\zerovec</m> for every vector <m>\vvec</m>,
	this means that <m>(qp)(T)=0</m>.
	</p>

	<p>This shows that there is a
	monic polynomial <m>s</m> such that <m>s(T)=0</m> on
	<m>V</m>.  Therefore, there is some possibly different
	polynomial having the smallest degree among all such
	polynomials, and this is the minimal
	polynomial of the operator <m>T</m> on <m>V</m>.
	</p>

	<p>To see that this polynomial is unique, suppose there are
	two monic polynomials <m>s_1</m> and <m>s_2</m> having
	smallest degree and <m>s_1(T)=0</m> and <m>s_2(T)=0</m>.
	If we consider <m>s_1-s_2</m>, we see that <m>\deg(s_1-s_2)\lt
	\deg(s_1)=\deg(s_2)</m> since the highest degree terms of
	<m>s_1</m> and <m>s_2</m> have coefficients <m>1</m> and
	therefore cancel.  Also,
	<me>
	  (s_1-s_2)(T) = s_1(T) - s_2(T) = 0
	</me>.
	However, this is impossible since <m>s_1</m> and <m>s_2</m>
	had the smallest possible degree among all polynomials that
	vanish when evaluated on <m>T</m>.  This means that
	<m>s_1=s_2</m>, which guarantees the uniqueness of the minimal
	polynomial. 
	</p>
      </proof>
    </theorem>

    <example xml:id="example-min-poly-1">
      <statement>
	<p> Consider the <m>2\times2</m> matrix 
	<m>A=\begin{bmatrix}
	2 \amp 0 \\
	0 \amp 2
	\end{bmatrix}</m> and the linear operator <m>T</m> that it
	defines.  Notice that <m>A-2I = 0</m> so if <m>p(x)=x-2</m>,
	then <m>p(T)=0</m>.  The minimal polynomial of <m>T</m> is
	therefore <m>p(x)=x-2</m>.
	</p>

	<p> More generally, suppose that the minimal polynomial of an
	operator <m>T</m> has degree <m>1</m>.  Since the minimal
	polynomial is monic, this means that <m>p(x)=x-\lambda</m>.
	Because <m>p(T)=T-\lambda I = 0</m>, we see that <m>T=\lambda
	I</m>, a multiple of the identity.
	</p>
      </statement>
    </example>

    <example xml:id="example-min-poly-2">
      <statement>
	<p> By contrast, consider the <m>2\times2</m> matrix 
	<m>B=\begin{bmatrix}
	2 &amp; 1 \\
	0 &amp; 2
	\end{bmatrix}</m> and the linear operator <m>S</m> that it
	defines with respect to some basis.  The degree of the minimal
	polynomial must be at least 2 since <m>B</m> is not a multiple
	of the identity matrix.  Notice, however, that 
	<m>B-2I = \begin{bmatrix}
	0 &amp; 1 \\
	0 &amp; 0 \\
	\end{bmatrix}
	</m> and <m>(B-2I)^2 = 0</m>.  This says that <m>(S-2I)^2 =
	0</m> and so the minimal polynomial of <m>S</m> is
	<m>q(x)=(x-2)^2</m>.
	</p>
      </statement>
    </example>

    <p> Both of the matrices in the two previous examples are
    upper triangular.  Remembering that the eigenvalues of an upper
    triangular matrix are the entries on the diagonal, we see that the
    roots of the minimal polynomials in both cases are the eigenvalues
    of the operator.  This gives some indication of the importance of
    the minimal polynomial, as we will see now.
    </p>

    <p>The fact that the minimal polynomial has the smallest degree
    among all polynomials for which <m>p(T)=0</m> has some important
    consequences. </p>

    <proposition xml:id="prop-min-poly-roots">
      <statement>
	<p>The set of roots of the minimal polynomial of <m>T</m>
	equals the set of eigenvalues of <m>T</m>.
	</p>
      </statement>

      <proof>
	<p>Suppose that <m>p</m> is the minimal polynomial of
	<m>T</m>.  We need to explain two things: that any eigenvalue
	of <m>T</m> is a root of <m>p</m> and that any root of
	<m>p</m> is an eigenvalue of <m>T</m>.
	</p>

	<p>Suppose that <m>\lambda</m> is an eigenvalue of <m>T</m>.
	This means that there is a nonzero vector <m>\vvec</m> such
	that <m>T\vvec = \lambda\vvec</m> and therefore <m>T^j\vvec =
	\lambda^j\vvec</m> for every <m>j</m>.  This means that
	<me>
	  0 = p(T)\vvec = p(\lambda)\vvec
	</me>,
	which implies that <m>p(\lambda) = 0</m>.  Therefore,
	<m>\lambda</m> is a root of <m>p</m>, the minimal polynomial
	of <m>T</m>.
	</p>

	<p>Conversely, suppose that <m>\lambda</m> is a root of
	<m>p</m>.  By <xref ref="prop-root-factor"/>, this means that
	<me>
	  p(x) = (x-\lambda)q(x)
	</me>.
	This says that
	<me>
	  0 = p(T) = (T-\lambda I)q(T)
	</me>
	However, <m>q(T)\neq 0</m> since <m>\deg(q) \lt \deg(p)</m>,
	there is some vector <m>\vvec</m> for which <m>q(T)\vvec\neq
	0</m>.  Therefore,
	<me>
	  0 = p(T)\vvec = (T-\lambda I)q(T)\vvec
	</me>,
	which shows that <m>q(T)\vvec</m> is an eigenvector <m>T</m>
	with associated eigenvalue <m>\lambda</m>.
	</p>
      </proof>
    </proposition>

    <p>This is the most significant fact about the minimal polynomial:
    that its roots are the eigenvalues of the operator.  We'll put
    this to use in the next section.  Before that, however, here are
    two other useful facts.
    </p>
    
    <proposition xml:id="prop-min-poly-div">
      <statement>
	<p>If <m>s</m> is a polynomial for which <m>s(T)=0</m>, then
	<m>s</m> is a multiple of the minimal polynomial of <m>T</m>.
	</p>
      </statement>
      <proof>
	<p>If <m>p</m> is the minimal polynomial of <m>T</m>, then 
	we can apply the Division Algorithm to write <m>s = pq + r</m>
	where <m>\deg(r) \lt \deg(p)</m>.  Furthermore,
	<me>
	  0 = s(T) = p(T)q(T) + r(T) = r(T)
	</me>,
	which implies that <m>r(T)=0</m>.  Since <m>p</m> has the
	smallest degree among all polynomials that vanish when
	evaluated on <m>T</m> and <m>r</m> has a smaller degree than
	<m>p</m>, we know that <m>r=0</m>.  Therefore, <m>s=pq</m>.
	</p>
      </proof>
    </proposition>

    <proposition xml:id="prop-min-poly-subspace">
      <statement>
	<p>If <m>T</m> is an operator on the vector space <m>V</m> and
	<m>W</m> is a subspace of <m>V</m> that is invariant under
	<m>T</m>, then the minimal polynomial of <m>T</m> is a
	multiple of the minimal polynomial of <m>T|_W</m>.
	</p>
      </statement>
      <proof>
	<p>Suppose that <m>s</m> is the minimal polynomial of
	<m>T|_W</m> and <m>p</m> is the minimal polynomial of <m>T</m>
	on <m>V</m>.  This means that <m>p(T)\wvec=0</m> 
	for every vector <m>\wvec</m> in <m>W</m> and so <m>p(T|_W) =
	0</m>.  We also know that <m>s</m> is the minimal polynomial
	of <m>T|_W</m> so by <xref ref="prop-min-poly-div"/>, we know
	that <m>p</m> is a multiple of <m>s</m>.
	</p>
      </proof>
    </proposition>

  </subsection>
</section>
